src/program_proof/lockservice/rpc_proof.v
@@ -4,7 +4,7 @@ From iris.program_logic Require Export weakestpre.
 From Perennial.algebra Require Import auth_map.
 From Perennial.goose_lang.lib Require Import lock.
 From Perennial.program_proof Require Import proof_prelude.
-From Perennial.program_proof.lockservice Require Import lockservice common_proof.
+From Perennial.program_proof.lockservice Require Import lockservice_nocrash common_proof.
 From Perennial.program_proof.lockservice Require Export rpc.
 
 Section rpc_proof.
